iris/BootChain.v
@@ -51,6 +51,7 @@ Require Import MbootVocab.
 Require Import MstatusFacts.
 Require Import KptPt.
 Require Import IntrDefs.
+Require Import WireInv.   (* [wire_inv] *)
 Require Import ProcGeom CpuOwn SchedCtx.
 Require Import SpecMain.
 Require Import BootConfig BootBridge PowerBoot.
@@ -711,6 +712,7 @@ Section BootPrimary.
     gen_cert -∗
     FsCrash.fs_crash_seam cov (FsImg.sb_logstart sb) -∗
     dev_inv γd γv -∗
+    wire_inv -∗
     uart_tx_own γd l0 -∗ uart_sent γd l0 -∗ uart_out_lb γd l0 -∗
     uart_dlab_is γd (DfracOwn (1/2)) b0 -∗
     disk_cfg_is γv (DfracOwn (1/2)) c0 -∗
@@ -724,7 +726,7 @@ Section BootPrimary.
     intros Hreset Hz Hprun Hlen Hlive Himg.
     iIntros "#Htext #Hdata Hres #Hstarted Hlk Hgl Hfirst Hnext Hpark Hpst Hpav
              Hfs Hmir Hirslot Hirauth #Hcert #Hseam
-             #Hdev Htx Hsent Hlb Hdlab Hcfg Hclaim #Hdone Hkpt Hkmap Hpages".
+             #Hdev #Hwire Htx Hsent Hlb Hdlab Hcfg Hclaim #Hdone Hkpt Hkmap Hpages".
     iApply (boot_entry_bridge rs iv dq Hreset with "Htext Hres").
     iIntros (mf) "Hcap Hctx Hcpu Hg Hraw #Htimc Hpc".
     iApply (Main.wp_main_boot_sconf mf (kv_frame_slots + K_main)%nat zero_reg ps
@@ -738,7 +740,7 @@ Section BootPrimary.
               with "Hcap Hctx Hcpu Hg Htext Hdata Hpc Hstarted [] Hlk Hgl
                     Hfirst Hnext Hpark Hpst Hpav Hfs Hmir Hirslot Hirauth
                     Hcert Hseam
-                    Hdev Htx Hsent Hlb Hdlab
+                    Hdev Hwire Htx Hsent Hlb Hdlab
                     Hcfg Hclaim Hdone Htimc Hraw Hkpt Hkmap Hpages").
     (* THE DEPOSIT WAND: main's boot arm hands over exactly [main_deposit]'s
        nine conjuncts at exactly its eight existential witnesses, so the wand
